extract rem4, containsProgram, old compile_lit code into separate files

compiler/src/FlatToRiscv.v
@@ -29,6 +29,9 @@ Require Import riscv.util.ZBitOps.
 Require Import compiler.util.Common.
 Require Import riscv.Utility.
 Require Import compiler.runsToNonDet.
+Require Import compiler.Rem4.
+Require Import compiler.containsProgram.
+
 
 (* TODO remove these three *)
 Require Import riscv.MachineWidth_XLEN.
@@ -65,6 +68,13 @@ Section RegisterFile.
     initialRegs := empty_map;
   |}.
 
+  Fixpoint setManyRegs(rf: RegisterFile Register mword)
+             (rnames: list Register)(vals: list mword): RegisterFile Register mword :=
+    match rnames, vals with
+    | x :: rnames, v :: vals => setReg (setManyRegs rf rnames vals) x v
+    | _, _ => rf
+    end.
+
 End RegisterFile.
 
 Existing Instance State_is_RegisterFile.
@@ -75,195 +85,6 @@ Section FlatToRiscv.
   Context {mword: Set}.
   Context {MW: MachineWidth mword}.
 
-  Ltac mword_cst w :=
-    match w with
-    | ZToReg ?x => let b := isZcst x in
-                  match b with
-                  | true => x
-                  | _ => constr:(NotConstant)
-                  end
-    | _ => constr:(NotConstant)
-  end.
-
-  Hint Rewrite
-    ZToReg_morphism.(morph_add)
-    ZToReg_morphism.(morph_sub)
-    ZToReg_morphism.(morph_mul)
-    ZToReg_morphism.(morph_opp)
-  : rew_ZToReg_morphism.
-
-  Add Ring mword_ring : (@regRing mword MW)
-      (preprocess [autorewrite with rew_ZToReg_morphism],
-       morphism (@ZToReg_morphism mword MW),
-       constants [mword_cst]).
-
-  Hint Rewrite @Zlength_nil @Zlength_cons @Zlength_app: rew_Zlength.
-
-  Ltac solve_word_eq :=
-    match goal with
-    | |- @eq mword _ _ => idtac
-    | _ => fail 1 "wrong shape of goal"
-    end;
-    subst;
-    try reflexivity;
-    clear;
-    simpl;
-    repeat (autorewrite with rew_Zlength; simpl);
-    try ring.
-
-  (* put here so that rem picks up the MachineWidth for wXLEN *)
-
-  (*
-  Lemma four_divides_Npow2_wXLEN:
-      exists k : N, (wordToN (natToWord wXLEN 4) * k)%N = Npow2 wXLEN.
-  Proof.
-    unfold wXLEN, bitwidth in *.
-    destruct Bw.
-    - exists (Npow2 30). reflexivity.
-    - exists (Npow2 62). reflexivity.
-  Qed.
-   *)
-
-  (* check lower two bits approach: how to connect to remu? or replace remu in spec? *)
-
-
-  Axiom euclid_unsigned: forall a b, a = add (mul (divu a b) b) (remu a b).
-  Axiom remu_range: forall (a b: mword), 0 <= regToZ_unsigned (remu a b) < regToZ_unsigned b.
-
-  Axiom unique: forall a b q r,
-      a = add (mul b q) r ->
-      0 <= regToZ_unsigned r < regToZ_unsigned b ->
-      q = divu a b /\ r = remu a b.
-
-  Definition divisibleBy4(a: mword): Prop := exists q, mul (ZToReg 4) q = a.
-
-  Lemma remu40_divisibleBy4: forall (a: mword),
-      remu a (ZToReg 4) = ZToReg 0 ->
-      divisibleBy4 a.
-  Proof.
-    intros.
-    unfold divisibleBy4.
-    exists (divu a (ZToReg 4)).
-    pose proof (euclid_unsigned a (ZToReg 4)) as P.
-    rewrite P at 2.
-    rewrite H.
-    ring.
-  Qed.
-
-  Lemma divisibleBy4_remu40: forall (a: mword),
-      divisibleBy4 a ->
-      remu a (ZToReg 4) = ZToReg 0.
-  Proof.
-    intros.
-    unfold divisibleBy4 in *.
-    destruct H as [q H].
-    destruct (@unique a (ZToReg 4) q (ZToReg 0)).
-    - subst a. ring.
-    - pose proof pow2_sz_4.
-      rewrite regToZ_ZToReg_unsigned by omega.
-      rewrite regToZ_ZToReg_unsigned by omega.
-      omega.
-    - congruence.
-  Qed.
-
-  Lemma remu_four_undo: forall a, remu (mul (ZToReg 4) a) (ZToReg 4) = ZToReg 0.
-  Proof.
-    intros.
-    rewrite remu_def.
-    f_equal.
-    pose proof pow2_sz_4.
-    rewrite mul_def_unsigned.
-    rewrite regToZ_ZToReg_unsigned_mod.
-    rewrite (regToZ_ZToReg_unsigned 4) by omega.
-    pose proof XLEN_lbound.
-    apply Z.rem_mod_eq_0; [omega|].
-    replace XLEN with (2 + (XLEN - 2)) by omega.
-    rewrite Z.pow_add_r by omega.
-    change (2 ^ 2) with 4.
-    pose proof (pow2_pos (XLEN - 2)).
-    div_mod_to_quot_rem. nia.
-  Qed.
-
-  Lemma remu_four_four: remu (ZToReg 4) (ZToReg 4) = ZToReg 0.
-  Proof.
-    intros.
-    apply divisibleBy4_remu40. unfold divisibleBy4.
-    exists (ZToReg 1). ring.
-  Qed.
-
-  Lemma remu_four_zero_distrib_plus: forall a b,
-      remu a (ZToReg 4) = ZToReg 0 ->
-      remu b (ZToReg 4) = ZToReg 0 ->
-      remu (add a b) (ZToReg 4) = ZToReg 0.
-  Proof.
-    intros.
-    apply divisibleBy4_remu40.
-    apply remu40_divisibleBy4 in H.  destruct H  as [q1 H1].
-    apply remu40_divisibleBy4 in H0. destruct H0 as [q2 H2].
-    unfold divisibleBy4 in *.
-    subst.
-    exists (add q1 q2).
-    ring.
-  Qed.
-
-  (* TODO is there a principled way of writing such proofs? *)
-  Lemma reduce_eq_to_sub_and_lt: forall (y z: mword) {T: Type} (thenVal elseVal: T),
-    (if ltu (sub y  z) (fromImm 1) then thenVal else elseVal) =
-    (if reg_eqb y z        then thenVal else elseVal).
-  Proof. (*
-    intros. destruct (weq y z).
-    - subst z. unfold wminus. rewrite wminus_inv.
-      destruct (wlt_dec (wzero wXLEN) $1); [reflexivity|].
-      change (wzero wXLEN) with (natToWord wXLEN 0) in n. unfold wlt in n.
-      exfalso. apply n.
-      do 2 rewrite wordToN_nat. rewrite roundTrip_0.
-      clear.
-      destruct wXLEN as [|w1] eqn: E.
-      + unfold wXLEN in *. destruct bitwidth; discriminate.
-      + rewrite roundTrip_1. simpl. constructor.
-    - destruct (@wlt_dec wXLEN (y ^- z) $ (1)) as [E|NE]; [|reflexivity].
-      exfalso. apply n. apply sub_0_eq.
-      unfold wlt in E.
-      do 2 rewrite wordToN_nat in E.
-      clear -E.
-      destruct wXLEN as [|w1] eqn: F.
-      + unfold wXLEN in *. destruct bitwidth; discriminate.
-      + rewrite roundTrip_1 in E.
-        simpl in E. apply N.lt_1_r in E. change 0%N with (N.of_nat 0) in E.
-        apply Nnat.Nat2N.inj in E. rewrite <- (roundTrip_0 (S w1)) in E.
-        apply wordToNat_inj in E.
-        exact E.
-  Qed.
-*)
-  Admitted.
-
-  (*
-  Lemma wlshift_bitSlice_plus: forall (sz1 sz2: Z) v,
-      (0 <= sz1)%Z ->
-      (0 <= sz2)%Z ->
-      wlshift (ZToWord wXLEN (bitSlice v sz1 (sz1 + sz2))) (Z.to_nat sz1)
-      ^+ ZToWord wXLEN (bitSlice v 0 sz1)
-      = ZToWord wXLEN (bitSlice v 0 (sz1 + sz2)).
-  Proof.
-    intros. rewrite wlshift_alt.
-    rewrite wlshift_mul_Zpow2 by assumption.
-    rewrite <- ZToWord_mult.
-    rewrite <- ZToWord_plus.
-    f_equal.
-    apply bitSlice_split; assumption.
-  Qed.
-  *)
-
-  (*
-  Context {Name: NameWithEq}.
-
-  (* If we made it a definition instead, destructing an if on "@dec (@eq (@var Name) x x0)"
-     (from this file), where a "@dec (@eq (@Reg Name) x x0)" (from another file, Riscv.v)
-     is in the context, will not recognize that these two are the same (they both reduce to
-     "@dec (@eq var x x0)", which is annoying. *)
-  Notation var := var.
-  Existing Instance eq_name_dec.
-   *)
 
   Context {stateMap: MapFunctions Register mword}.
   Notation locals := (map Register mword).
@@ -328,6 +149,128 @@ Section FlatToRiscv.
       (regToZ_unsigned a) mod 8 = 0 ->
       translate mode (ZToReg 8) a = Return a.
 
+  Variable LwXLEN: Register -> Register -> Z -> Instruction.
+
+  Variable SwXLEN: Register -> Register -> Z -> Instruction.
+
+  Variable compile_ext_call: list var -> Action -> list var -> list Instruction.
+  Hypothesis compile_ext_call_length: forall binds f args,
+      Zlength (compile_ext_call binds f args) <= 7. (* TODO parametrize *)
+
+
+  Hypothesis compile_ext_call_correct: forall initialL action outcome post newPc insts
+      (argvars resvars: list var),
+      insts = compile_ext_call resvars action argvars ->
+      newPc = add initialL.(getPc) (ZToReg (4 * Zlength insts)) ->
+      containsProgram initialL.(getMem) insts initialL.(getPc) ->
+      ext_spec action initialL.(getLog) (List.map (getReg (initialL.(getRegs))) argvars)
+               outcome ->
+      (forall newLog resvals,
+          outcome newLog resvals ->
+          runsTo RiscvMachineL (mcomp_sat (run1 (B := BitWidth))) {|
+            getRegs   := setManyRegs initialL.(getRegs) resvars resvals;
+            getPc     := newPc;
+            getNextPc := add newPc (ZToReg 4);
+            getMem    := initialL.(getMem);
+            getLog    := newLog;
+          |} post) ->
+      runsTo RiscvMachineL (mcomp_sat (run1 (B := BitWidth))) initialL post.
+
+  Ltac mword_cst w :=
+    match w with
+    | ZToReg ?x => let b := isZcst x in
+                  match b with
+                  | true => x
+                  | _ => constr:(NotConstant)
+                  end
+    | _ => constr:(NotConstant)
+  end.
+
+  Hint Rewrite
+    ZToReg_morphism.(morph_add)
+    ZToReg_morphism.(morph_sub)
+    ZToReg_morphism.(morph_mul)
+    ZToReg_morphism.(morph_opp)
+  : rew_ZToReg_morphism.
+
+  Add Ring mword_ring : (@regRing mword MW)
+      (preprocess [autorewrite with rew_ZToReg_morphism],
+       morphism (@ZToReg_morphism mword MW),
+       constants [mword_cst]).
+
+  Hint Rewrite @Zlength_nil @Zlength_cons @Zlength_app: rew_Zlength.
+
+  Ltac solve_word_eq :=
+    match goal with
+    | |- @eq mword _ _ => idtac
+    | _ => fail 1 "wrong shape of goal"
+    end;
+    subst;
+    try reflexivity;
+    clear;
+    simpl;
+    repeat (autorewrite with rew_Zlength; simpl);
+    try ring.
+
+  (* TODO is there a principled way of writing such proofs? *)
+  Lemma reduce_eq_to_sub_and_lt: forall (y z: mword) {T: Type} (thenVal elseVal: T),
+    (if ltu (sub y  z) (fromImm 1) then thenVal else elseVal) =
+    (if reg_eqb y z        then thenVal else elseVal).
+  Proof. (*
+    intros. destruct (weq y z).
+    - subst z. unfold wminus. rewrite wminus_inv.
+      destruct (wlt_dec (wzero wXLEN) $1); [reflexivity|].
+      change (wzero wXLEN) with (natToWord wXLEN 0) in n. unfold wlt in n.
+      exfalso. apply n.
+      do 2 rewrite wordToN_nat. rewrite roundTrip_0.
+      clear.
+      destruct wXLEN as [|w1] eqn: E.
+      + unfold wXLEN in *. destruct bitwidth; discriminate.
+      + rewrite roundTrip_1. simpl. constructor.
+    - destruct (@wlt_dec wXLEN (y ^- z) $ (1)) as [E|NE]; [|reflexivity].
+      exfalso. apply n. apply sub_0_eq.
+      unfold wlt in E.
+      do 2 rewrite wordToN_nat in E.
+      clear -E.
+      destruct wXLEN as [|w1] eqn: F.
+      + unfold wXLEN in *. destruct bitwidth; discriminate.
+      + rewrite roundTrip_1 in E.
+        simpl in E. apply N.lt_1_r in E. change 0%N with (N.of_nat 0) in E.
+        apply Nnat.Nat2N.inj in E. rewrite <- (roundTrip_0 (S w1)) in E.
+        apply wordToNat_inj in E.
+        exact E.
+  Qed.
+*)
+  Admitted.
+
+  (*
+  Lemma wlshift_bitSlice_plus: forall (sz1 sz2: Z) v,
+      (0 <= sz1)%Z ->
+      (0 <= sz2)%Z ->
+      wlshift (ZToWord wXLEN (bitSlice v sz1 (sz1 + sz2))) (Z.to_nat sz1)
+      ^+ ZToWord wXLEN (bitSlice v 0 sz1)
+      = ZToWord wXLEN (bitSlice v 0 (sz1 + sz2)).
+  Proof.
+    intros. rewrite wlshift_alt.
+    rewrite wlshift_mul_Zpow2 by assumption.
+    rewrite <- ZToWord_mult.
+    rewrite <- ZToWord_plus.
+    f_equal.
+    apply bitSlice_split; assumption.
+  Qed.
+  *)
+
+  (*
+  Context {Name: NameWithEq}.
+
+  (* If we made it a definition instead, destructing an if on "@dec (@eq (@var Name) x x0)"
+     (from this file), where a "@dec (@eq (@Reg Name) x x0)" (from another file, Riscv.v)
+     is in the context, will not recognize that these two are the same (they both reduce to
+     "@dec (@eq var x x0)", which is annoying. *)
+  Notation var := var.
+  Existing Instance eq_name_dec.
+   *)
+
   (* This phase assumes that register allocation has already been done on the FlatImp
      level, and expects the following to hold: *)
   Fixpoint valid_registers(s: stmt): Prop :=
@@ -345,19 +288,9 @@ Section FlatToRiscv.
     | SInteract binds _ args => Forall valid_register binds /\ Forall valid_register args (* untested *)
     end.
 
-  (*
-  Variable var2Register: var -> Register. (* TODO register allocation *)
-  Hypothesis no_var_mapped_to_Register0: forall (x: var), x <> Register0.
-  Hypothesis var2Register_inj: forall x1 x2, x1 = x2 -> x1 = x2.
-   *)
-
   (* Set Printing Projections.
      Uncaught anomaly when stepping through proofs :(
      https://github.com/coq/coq/issues/6257 *)
-
-  Variable LwXLEN: Register -> Register -> Z -> Instruction.
-
-  Variable SwXLEN: Register -> Register -> Z -> Instruction.
 
   Definition compile_op(rd: Register)(op: bopname)(rs1 rs2: Register): list Instruction :=
     match op with
@@ -400,130 +333,6 @@ Section FlatToRiscv.
 
   Definition compile_lit(rd: Register)(v: Z): list Instruction :=
     compile_lit_rec 7 rd Register0 v.
-
-  Definition compile_lit_32(rd: Register)(v: word 32): list Instruction :=
-    let h0 := wsplit_lo 16 16 v in
-    let h1 := wsplit_hi 16 16 v in
-    [[Addi rd Register0 (uwordToZ h1); Slli rd rd 16; Addi rd rd (uwordToZ h0)]].
-
-  Definition compile_lit_64(rd: Register)(v: word 64): list Instruction :=
-    let w0 := wsplit_lo 32 32 v in
-    let w1 := wsplit_hi 32 32 v in
-    let h0 := wsplit_lo 16 16 w0 in
-    let h1 := wsplit_hi 16 16 w0 in
-    let h2 := wsplit_lo 16 16 w1 in
-    let h3 := wsplit_hi 16 16 w1 in
-    [[Addi rd Register0 (uwordToZ h3);
-      Slli rd rd 16; Addi rd rd (uwordToZ h2);
-      Slli rd rd 16; Addi rd rd (uwordToZ h1);
-      Slli rd rd 16; Addi rd rd (uwordToZ h0)]].
-
-  (* The problem with the primed version is that we have to destruct the bitwidth to expose
-     the indivdual commands (on which the proof machinery of compile_stmt_correct_aux works),
-     but the proof machinery stops working when the bitwidth is destructed because typeclass
-     search stops working as it should, and destructing the bitwidth only works after unfolding
-     all definitions involving mword.
-  Definition compile_lit'(rd: Register)(v: mword): list Instruction.
-    clear -Bw rd v. unfold wXLEN, bitwidth in *. destruct Bw.
-    - exact (compile_lit_32 rd v).
-    - exact (compile_lit_64 rd v).
-  Defined.
-
-  (* Very stupid workaround: *)
-  Definition make_64_bit(v: mword): word 64.
-    clear -Bw v. unfold wXLEN, bitwidth in *. destruct Bw.
-    - exact (zext v 32).
-    - exact v.
-  Defined.
-
-  Definition compile_lit''(rd: Register)(v: mword): list Instruction :=
-    compile_lit_64 rd (make_64_bit v).
-
-  (* store the n lowest halves (1 half = 16bits) of v into rd *)
-  Fixpoint compile_halves(n: nat)(rd: Register)(v: Z): list Instruction :=
-    if dec (- 2^19 <= v < 2^19)%Z then
-      [[Addi rd Register0 v]]
-    else
-      match n with
-      | O => [[]] (* will not happen because we choose n big enough *)
-      | S n' =>
-        let upper := (v / 2^16)%Z in
-        let lower := (v - upper * 2^16)%Z in
-        (compile_halves n' rd upper) ++ [[Slli rd rd 16; Addi rd rd lower]]
-      end.
-
-  Fixpoint interp_compiled_halves(l: list Instruction)(acc: Z): Z :=
-    match l with
-    | (Addi _ _ v) :: l' => interp_compiled_halves l' (acc + v)
-    | (Slli _ _ _) :: l' => interp_compiled_halves l' (acc * 16)
-    | _ => acc
-    end.
-
-  Lemma compile_halves_correct: forall n rd v acc,
-      v <=2^(16 * n)
-      interp_compiled_halves (compile_halves n rd v) acc = (acc + v)%Z.
-  Proof.
-    induction n; intros.
-    - simpl.
-  Qed.
-
-  Definition compile_lit_old(rd: Register)(v: Z): list Instruction :=
-    compile_halves (wXLEN / 16) rd v.
-
-  Definition add_lit_20(rd rs: Register)(v: word 20): list Instruction :=
-    [[Addi rd rs (wordToZ v)]].
-
-  Definition add_lit_32(rd rs: Register)(v: word 32): list Instruction :=
-    let lobits := split1 20 12 v in
-    let hibits := split2 20 12 v in [[]].
-
-  Definition embed_words(l: list (word 32)): list Instruction :=
-    [[J (Z.of_nat (length l))]] ++ (map (fun w => InvalidInstruction (wordToZ w)) l).
-
-  Definition wXLEN_to_word_list(v: mword): list (word 32).
-    clear -Bw v. unfold wXLEN, bitwidth in *. destruct Bw.
-    - exact [v].
-    - exact [split1 32 32 v; split2 32 32 v].
-  Defined.
-
-  Definition embed_word(v: mword): list Instruction :=
-    List.map (fun w => InvalidInstruction (wordToZ w)) (wXLEN_to_word_list v).
-
-  Definition compile_lit_old1(rd: Register)(v: mword): list Instruction :=
-    let l := embed_word v in
-    [[Auipc rd 0; LwXLEN rd rd 8; J (Z.of_nat (length l))]] ++ l.
-
-  Definition add_lit_20'(rd rs: Register)(v: Z): list Instruction :=
-    [[Addi rd rs v]].
-
-  Definition add_lit_32'(rd rs: Register)(v: Z): list Instruction :=
-    (if dec (- 2^19 <= v < 2^19)%Z then [[]] else (
-         let '(hibits, lobits) := (1%Z, 1%Z) in
-         let maybe1 := 1%Z in
-         ([[ Lui rd hibits ]] ++ (add_lit_20' rd rs (lobits + maybe1))))).
-
-  Definition compile_lit_32(rd: Register)(v: Z): list Instruction :=
-      let lobits := (v mod (2 ^ 20))%Z in
-      if dec (lobits = v)
-      then [[Addi rd Register0 lobits]]
-      else
-        let hibits := (v - lobits)%Z in
-        if Z.testbit v 20
-        (* Xori will sign-extend lobits with 1s, therefore Z.lnot *)
-        then [[Lui rd (Z.lnot hibits); Xori rd rd lobits]]
-        (* Xori will sign-extend lobits with 0s *)
-        else [[Lui rd hibits; Xori rd rd lobits]].
-
-  Definition compile_lit_old'(rd: Register)(v: mword): list Instruction.
-    clear -Bw rd v. unfold wXLEN, bitwidth in *. destruct Bw.
-    - exact (compile_lit_32 rd v).
-    - exact (compile_lit_64 rd v).
-  Defined.
-  *)
-
-  Variable compile_ext_call: list var -> Action -> list var -> list Instruction.
-  Hypothesis compile_ext_call_length: forall binds f args,
-      Zlength (compile_ext_call binds f args) <= 7. (* TODO parametrize *)
 
   Fixpoint compile_stmt(s: stmt): list (Instruction) :=
     match s with
@@ -579,60 +388,8 @@ Section FlatToRiscv.
       omega.
   Qed.
 
-  (* load and decode Inst *)
-  Definition ldInst(m: Mem mword)(a: mword): Instruction :=
-    decode (@RV_wXLEN_IM BitWidth) (uwordToZ (Memory.loadWord m a)).
-
-  Definition decode_prog(prog: list (word 32)): list Instruction :=
-    List.map (fun w => decode (@RV_wXLEN_IM BitWidth) (uwordToZ w)) prog.
-
   Definition mem_inaccessible(m: Memory.mem)(start len: Z): Prop :=
     forall a w, Memory.read_mem a m = Some w -> not_in_range a XLEN_in_bytes start len.
-
-  Definition containsProgram(m: Mem mword)(program: list Instruction)(offset: mword) :=
-    regToZ_unsigned offset + 4 * Zlength program <= Memory.memSize m /\
-    forall i inst, Znth_error program i = Some inst ->
-      ldInst m (add offset (ZToReg (4 * i))) = inst.
-
-  Definition containsProgram'(m: Mem mword)(program: list Instruction)(offset: mword) :=
-    regToZ_unsigned offset + 4 * Zlength program <= Memory.memSize m /\
-    decode_prog (Memory.load_word_list m offset (Zlength program)) = program.
-
-  Lemma containsProgram_alt: forall m program offset,
-      containsProgram m program offset <-> containsProgram' m program offset.
-  Proof.
-    intros. unfold containsProgram, containsProgram', decode_prog.
-    clear LwXLEN SwXLEN.
-    intuition idtac.
-    - apply list_elementwise_same_Z. intros i B. specialize (H1 i).
-      assert (0 <= i < Zlength program \/ Zlength program <= i) as C by omega.
-      destruct C as [C | C].
-      + destruct (Znth_error_Some _ program i) as [_ P].
-        specialize (P C).
-        destruct (Znth_error program i) as [inst|] eqn: E; try contradiction.
-        specialize (H1 _ eq_refl). unfold ldInst in H1.
-        erewrite map_Znth_error.
-        * f_equal. eassumption.
-        * apply Znth_error_load_word_list; try assumption.
-      + pose proof (Znth_error_ge_None _ _ C) as P.
-        rewrite P.
-        apply Znth_error_ge_None.
-        rewrite map_Zlength.
-        rewrite Zlength_load_word_list by (apply Zlength_nonneg).
-        assumption.
-    - unfold ldInst. rewrite <- H1 in H.
-      pose proof (map_Znth_error') as P.
-      specialize P with (1 := H).
-      destruct P as [inst' [P Q] ].
-      subst inst.
-      do 2 f_equal.
-      rewrite Znth_error_load_word_list in P.
-      + congruence.
-      + edestruct (Znth_error_Some _ (Memory.load_word_list m offset (Zlength program)))
-          as [Q _].
-        rewrite Zlength_load_word_list in Q by (apply Zlength_nonneg).
-        apply Q. congruence.
-  Qed.
 
   Lemma nth_error_nil_Some: forall {A} i (a: A), nth_error nil i = Some a -> False.
   Proof.
@@ -668,181 +425,6 @@ Section FlatToRiscv.
     nat_rel_with_words_pre(*;
     nat_div_mod_to_quot_rem;
     nia *).
-
-  (* Note: containsProgram for one single [[inst]] could be simplified, but for automation,
-     it's better not to simplify.
-  Lemma containsProgram_cons_inv_old: forall m inst insts offset,
-    containsProgram m (inst :: insts) offset ->
-    containsProgram m [[inst]] offset /\
-    containsProgram m insts (add offset ZToReg 4).
-  Proof.
-    intros *. intro Cp. unfold containsProgram in *. cbn [length] in *.
-    intuition (try omega).
-    + specialize (H0 0). specialize H0 with (1 := eq_refl).
-      intros. destruct i; inverts H1.
-      - assumption.
-      - exfalso. eauto using nth_error_nil_Some.
-    + nat_rel_with_words.
-    + rename H0 into Cp. specialize (Cp (S i)). simpl in Cp.
-      specialize (Cp _ H1).
-      rewrite <- Cp. f_equal.
-      solve_word_eq.
-  Qed.
-  *)
-
-  Definition containsProgram_app_will_work(insts1 insts2: list Instruction)(offset: mword) :=
-    (regToZ_unsigned (mul (add offset (ZToReg 4)) (ZToReg (Zlength insts1))) = 0 ->
-     insts1 = nil \/ insts2 = nil).
-
-  Lemma containsProgram_app_inv0: forall s insts1 insts2 offset,
-    containsProgram s (insts1 ++ insts2) offset ->
-    containsProgram s insts1 offset /\
-    containsProgram s insts2 (add offset (ZToReg (4 * Zlength insts1))) /\
-    containsProgram_app_will_work insts1 insts2 offset.
-  Proof.
-  (*
-    intros *. intro Cp. unfold containsProgram, containsProgram_app_will_work in *.
-    rewrite app_length in Cp.
-    intuition (try nat_rel_with_words).
-    + apply H0. rewrite nth_error_app1; [assumption|].
-      apply nth_error_Some. intro E. rewrite E in H1. discriminate.
-    + rewrite <- (H0 (length insts1 + i)).
-      - f_equal. solve_word_eq.
-      - rewrite nth_error_app2 by omega.
-        replace (length insts1 + i - length insts1) with i by omega.
-        assumption.
-    + destruct insts2; [solve [auto]|].
-      destruct insts1; [solve [auto]|].
-      exfalso.
-      simpl (length _) in *.
-      rewrite Nat.mul_add_distr_l in H.
-      rewrite Nat.add_assoc in H.
-      rewrite wordToNat_wplus in H1.
-      rewrite? wordToNat_wmult in *.
-      rewrite? wordToNat_natToWord_eqn in *.
-      pose proof pow2_wXLEN_4.
-      rewrite Nat.add_mod in H1 by omega.
-      rewrite <- Nat.mul_mod in * by omega.
-      rewrite Nat.add_mod_idemp_r in H1 by omega.
-      rewrite <- Nat.add_mod in H1 by omega.
-      pose proof (Memory.memSize_bound s).
-      rewrite Nat.mod_small in H1 by omega.
-      clear -H1. omega.
-  Qed.
-   *)
-  Admitted.
-
-  Lemma containsProgram_app_inv: forall s insts1 insts2 offset,
-    containsProgram s (insts1 ++ insts2) offset ->
-    containsProgram s insts1 offset /\
-    containsProgram s insts2 (add offset (mul (ZToReg 4) (ZToReg (Zlength insts1)))) /\
-    containsProgram_app_will_work insts1 insts2 offset.
-  Proof.
-    intros.
-    destruct (containsProgram_app_inv0 _ _ H) as [H1 H2].
-    rewrite ZToReg_morphism.(morph_mul) in H2.
-    rewrite <- regToZ_unsigned_four in H2.
-    rewrite ZToReg_regToZ_unsigned in H2.
-    auto.
-  Qed.
-
-  Lemma containsProgram_cons_inv: forall m inst insts offset,
-    containsProgram m (inst :: insts) offset ->
-    containsProgram m [[inst]] offset /\
-    containsProgram m insts (add offset (ZToReg 4)) /\
-    containsProgram_app_will_work [[inst]] insts offset.
-  Proof.
-    intros.
-    pose proof containsProgram_app_inv as P.
-    specialize P with (insts1 := [[inst]]) (insts2 := insts).
-    (* TODO how to automate this nicely? "match" and equate? *)
-    replace (add offset (ZToReg 4)) with (add offset (mul (ZToReg 4) (ZToReg (Zlength [[inst]])))); auto.
-    rewrite Zlength_cons. rewrite Zlength_nil.
-    change (0 + 1) with 1.
-    rewrite <- regToZ_unsigned_one.
-    simpl in *.
-    rewrite ZToReg_regToZ_unsigned.
-    ring.
-  Qed.
-
-  Lemma containsProgram_app: forall m insts1 insts2 offset,
-      containsProgram_app_will_work insts1 insts2 offset ->
-      containsProgram m insts1 offset ->
-      containsProgram m insts2 (add offset (mul (ZToReg 4) (ZToReg (Zlength insts1)))) ->
-      containsProgram m (insts1 ++ insts2) offset.
-  Proof.
-    (*
-    unfold containsProgram, containsProgram_app_will_work.
-    intros *. intro A. intros. rewrite app_length.
-    intuition idtac.
-    - clear H2 H3.
-      repeat match goal with
-             | IsMem: Memory.Memory ?M _, m: ?M |- _ =>
-               unique pose proof (@Memory.memSize_bound M _ IsMem m)
-             end.
-      pose proof pow2_wXLEN_4.
-      assert (let x := regToZ_unsigned  (offset ^+ $ (4) ^* $ (length insts1)) in x = 0 \/ x > 0) as C
-        by (cbv zeta; omega).
-      destruct C as [C | C].
-      + specialize (A C). destruct A as [A | A].
-        * subst insts1.
-          change (length [[]]) with 0 in *.
-          rewrite Nat.add_0_l.
-          replace (offset ^+ $ (4) ^* $ (0)) with offset in C by solve_word_eq.
-          apply wordToNat_zero in C. subst offset.
-          rewrite roundTrip_0 in *.
-          match goal with
-          | H: regToZ_unsigned ?b + 4 * length insts2 <= _ |- _ =>
-            replace 0 with (regToZ_unsigned b) at 1; [assumption|]
-          end.
-          rewrite <- roundTrip_0 at 4.
-          f_equal.
-          solve_word_eq.
-        * subst insts2.
-          change (length [[]]) with 0.
-          rewrite Nat.add_0_r.
-          assumption.
-      + repeat match goal with
-             | IsMem: Memory.Memory ?M _, m: ?M |- _ =>
-               unique pose proof (@Memory.memSize_bound M _ IsMem m)
-             end.
-        pose proof pow2_wXLEN_4.
-        rewrite? wordToNat_wplus in *.
-        rewrite? wordToNat_natToWord_eqn in *.
-        rewrite? wordToNat_wmult in *.
-        rewrite? wordToNat_natToWord_eqn in *.
-        rewrite <- Nat.mul_mod in * by omega.
-        rewrite Nat.add_mod_idemp_r in * by omega.
-        nat_div_mod_to_quot_rem.
-        assert (q = 0 \/ q > 0) as D by omega.
-        destruct D as [D | D]; nia.
-    - assert (i < length insts1 \/ length insts1 <= i) as E by omega.
-      destruct E as [E | E].
-      + rewrite nth_error_app1 in H0 by assumption. eauto.
-      + rewrite nth_error_app2 in H0 by assumption.
-        erewrite <- H3; [|exact H0].
-        f_equal.
-        replace i with (i - length insts1 + length insts1) at 1 by omega.
-        forget (i - length insts1) as i'.
-        solve_word_eq.
-  Qed.*)
-  Admitted.
-
-  Lemma containsProgram_cons: forall m inst insts offset,
-    containsProgram_app_will_work [[inst]] insts offset ->
-    containsProgram m [[inst]] offset ->
-    containsProgram m insts (add offset (ZToReg 4)) ->
-    containsProgram m (inst :: insts) offset.
-  Proof.
-    intros. change (inst :: insts) with ([[inst]] ++ insts).
-    apply containsProgram_app; [assumption..|].
-    rewrite Zlength_cons, Zlength_nil.
-    repeat match goal with
-           | H: containsProgram _ _ ?x |- _ => progress (ring_simplify x in H)
-           | |-  containsProgram _ _ ?x     => progress (ring_simplify x)
-           end.
-    assumption.
-  Qed.
 
   Arguments containsProgram: simpl never.
 
@@ -1832,31 +1414,6 @@ Section FlatToRiscv.
     f_equal; try solve_word_eq.
     f_equal. symmetry. apply compile_lit_correct.
   Qed.
-
-  Fixpoint setManyRegs(rf: RegisterFile Register mword)
-             (rnames: list Register)(vals: list mword): RegisterFile Register mword :=
-    match rnames, vals with
-    | x :: rnames, v :: vals => setReg (setManyRegs rf rnames vals) x v
-    | _, _ => rf
-    end.
-
-  Hypothesis compile_ext_call_correct: forall initialL action outcome post newPc insts
-      (argvars resvars: list var),
-      insts = compile_ext_call resvars action argvars ->
-      newPc = add initialL.(getPc) (ZToReg (4 * Zlength insts)) ->
-      containsProgram initialL.(getMem) insts initialL.(getPc) ->
-      ext_spec action initialL.(getLog) (List.map (getReg (initialL.(getRegs))) argvars)
-               outcome ->
-      (forall newLog resvals,
-          outcome newLog resvals ->
-          runsTo {|
-            getRegs   := setManyRegs initialL.(getRegs) resvars resvals;
-            getPc     := newPc;
-            getNextPc := add newPc (ZToReg 4);
-            getMem    := initialL.(getMem);
-            getLog    := newLog;
-          |} post) ->
-      runsTo initialL post.
 
   (* COQBUG(unification finds Type instead of Prop and fails to downgrade *)
   Implicit Types post : trace -> @Memory.mem mword -> locals -> Prop.
