compiler/src/FlatToRiscv32Specifics.v
@@ -15,3 +15,125 @@ Instance FlatToRiscv32Specifics{MW: MachineWidth (word 32)}{MF: MemoryFunctions 
   storeWordwXLEN := storeWord;
 
 |}.
+
+(* old compile_lit code, TODO reactivate
+
+  Definition compile_lit_32(rd: Register)(v: word 32): list Instruction :=
+    let h0 := wsplit_lo 16 16 v in
+    let h1 := wsplit_hi 16 16 v in
+    [[Addi rd Register0 (uwordToZ h1); Slli rd rd 16; Addi rd rd (uwordToZ h0)]].
+
+  Definition compile_lit_64(rd: Register)(v: word 64): list Instruction :=
+    let w0 := wsplit_lo 32 32 v in
+    let w1 := wsplit_hi 32 32 v in
+    let h0 := wsplit_lo 16 16 w0 in
+    let h1 := wsplit_hi 16 16 w0 in
+    let h2 := wsplit_lo 16 16 w1 in
+    let h3 := wsplit_hi 16 16 w1 in
+    [[Addi rd Register0 (uwordToZ h3);
+      Slli rd rd 16; Addi rd rd (uwordToZ h2);
+      Slli rd rd 16; Addi rd rd (uwordToZ h1);
+      Slli rd rd 16; Addi rd rd (uwordToZ h0)]].
+
+     The problem with the primed version is that we have to destruct the bitwidth to expose
+     the indivdual commands (on which the proof machinery of compile_stmt_correct_aux works),
+     but the proof machinery stops working when the bitwidth is destructed because typeclass
+     search stops working as it should, and destructing the bitwidth only works after unfolding
+     all definitions involving mword.
+  Definition compile_lit'(rd: Register)(v: mword): list Instruction.
+    clear -Bw rd v. unfold wXLEN, bitwidth in *. destruct Bw.
+    - exact (compile_lit_32 rd v).
+    - exact (compile_lit_64 rd v).
+  Defined.
+
+  (* Very stupid workaround: *)
+  Definition make_64_bit(v: mword): word 64.
+    clear -Bw v. unfold wXLEN, bitwidth in *. destruct Bw.
+    - exact (zext v 32).
+    - exact v.
+  Defined.
+
+  Definition compile_lit''(rd: Register)(v: mword): list Instruction :=
+    compile_lit_64 rd (make_64_bit v).
+
+  (* store the n lowest halves (1 half = 16bits) of v into rd *)
+  Fixpoint compile_halves(n: nat)(rd: Register)(v: Z): list Instruction :=
+    if dec (- 2^19 <= v < 2^19)%Z then
+      [[Addi rd Register0 v]]
+    else
+      match n with
+      | O => [[]] (* will not happen because we choose n big enough *)
+      | S n' =>
+        let upper := (v / 2^16)%Z in
+        let lower := (v - upper * 2^16)%Z in
+        (compile_halves n' rd upper) ++ [[Slli rd rd 16; Addi rd rd lower]]
+      end.
+
+  Fixpoint interp_compiled_halves(l: list Instruction)(acc: Z): Z :=
+    match l with
+    | (Addi _ _ v) :: l' => interp_compiled_halves l' (acc + v)
+    | (Slli _ _ _) :: l' => interp_compiled_halves l' (acc * 16)
+    | _ => acc
+    end.
+
+  Lemma compile_halves_correct: forall n rd v acc,
+      v <=2^(16 * n)
+      interp_compiled_halves (compile_halves n rd v) acc = (acc + v)%Z.
+  Proof.
+    induction n; intros.
+    - simpl.
+  Qed.
+
+  Definition compile_lit_old(rd: Register)(v: Z): list Instruction :=
+    compile_halves (wXLEN / 16) rd v.
+
+  Definition add_lit_20(rd rs: Register)(v: word 20): list Instruction :=
+    [[Addi rd rs (wordToZ v)]].
+
+  Definition add_lit_32(rd rs: Register)(v: word 32): list Instruction :=
+    let lobits := split1 20 12 v in
+    let hibits := split2 20 12 v in [[]].
+
+  Definition embed_words(l: list (word 32)): list Instruction :=
+    [[J (Z.of_nat (length l))]] ++ (map (fun w => InvalidInstruction (wordToZ w)) l).
+
+  Definition wXLEN_to_word_list(v: mword): list (word 32).
+    clear -Bw v. unfold wXLEN, bitwidth in *. destruct Bw.
+    - exact [v].
+    - exact [split1 32 32 v; split2 32 32 v].
+  Defined.
+
+  Definition embed_word(v: mword): list Instruction :=
+    List.map (fun w => InvalidInstruction (wordToZ w)) (wXLEN_to_word_list v).
+
+  Definition compile_lit_old1(rd: Register)(v: mword): list Instruction :=
+    let l := embed_word v in
+    [[Auipc rd 0; LwXLEN rd rd 8; J (Z.of_nat (length l))]] ++ l.
+
+  Definition add_lit_20'(rd rs: Register)(v: Z): list Instruction :=
+    [[Addi rd rs v]].
+
+  Definition add_lit_32'(rd rs: Register)(v: Z): list Instruction :=
+    (if dec (- 2^19 <= v < 2^19)%Z then [[]] else (
+         let '(hibits, lobits) := (1%Z, 1%Z) in
+         let maybe1 := 1%Z in
+         ([[ Lui rd hibits ]] ++ (add_lit_20' rd rs (lobits + maybe1))))).
+
+  Definition compile_lit_32(rd: Register)(v: Z): list Instruction :=
+      let lobits := (v mod (2 ^ 20))%Z in
+      if dec (lobits = v)
+      then [[Addi rd Register0 lobits]]
+      else
+        let hibits := (v - lobits)%Z in
+        if Z.testbit v 20
+        (* Xori will sign-extend lobits with 1s, therefore Z.lnot *)
+        then [[Lui rd (Z.lnot hibits); Xori rd rd lobits]]
+        (* Xori will sign-extend lobits with 0s *)
+        else [[Lui rd hibits; Xori rd rd lobits]].
+
+  Definition compile_lit_old'(rd: Register)(v: mword): list Instruction.
+    clear -Bw rd v. unfold wXLEN, bitwidth in *. destruct Bw.
+    - exact (compile_lit_32 rd v).
+    - exact (compile_lit_64 rd v).
+  Defined.
+  *)
