compiler/src/containsProgram.v
@@ -1,0 +1,279 @@
+Require Import Coq.Lists.List.
+Import ListNotations.
+Require Import Coq.ZArith.ZArith.
+Require Import bbv.ZLib.
+Require Import riscv.Decode.
+Require Import riscv.Run.
+Require Import riscv.Memory.
+Require Import compiler.Decidable.
+Require compiler.Memory.
+Require Import Coq.Program.Tactics.
+Require Import riscv.InstructionCoercions.
+Require Import riscv.AxiomaticRiscv.
+Require Import Coq.micromega.Lia.
+Require Import riscv.Utility.
+Require Import compiler.FlatToRiscvBitWidthSpecifics.
+
+Local Open Scope ilist_scope.
+Local Open Scope Z_scope.
+
+Set Implicit Arguments.
+
+
+Section ContainsProgram.
+
+  Context {mword: Set}.
+  Context {MW: MachineWidth mword}.
+  Context {MF: Memory.MemoryFunctions mword}.
+  Context {BWS: FlatToRiscvBitWidthSpecifics mword}.
+
+  Ltac mword_cst w :=
+    match w with
+    | ZToReg ?x => let b := isZcst x in
+                  match b with
+                  | true => x
+                  | _ => constr:(NotConstant)
+                  end
+    | _ => constr:(NotConstant)
+  end.
+
+  Hint Rewrite
+    ZToReg_morphism.(morph_add)
+    ZToReg_morphism.(morph_sub)
+    ZToReg_morphism.(morph_mul)
+    ZToReg_morphism.(morph_opp)
+  : rew_ZToReg_morphism.
+
+  Add Ring mword_ring : (@regRing mword MW)
+      (preprocess [autorewrite with rew_ZToReg_morphism],
+       morphism (@ZToReg_morphism mword MW),
+       constants [mword_cst]).
+
+
+  (* load and decode Inst *)
+  Definition ldInst(m: Mem mword)(a: mword): Instruction :=
+    decode (@RV_wXLEN_IM BitWidth) (uwordToZ (Memory.loadWord m a)).
+
+  Definition decode_prog(prog: list (word 32)): list Instruction :=
+    List.map (fun w => decode (@RV_wXLEN_IM BitWidth) (uwordToZ w)) prog.
+
+  Definition containsProgram(m: Mem mword)(program: list Instruction)(offset: mword) :=
+    regToZ_unsigned offset + 4 * Zlength program <= Memory.memSize m /\
+    forall i inst, Znth_error program i = Some inst ->
+      ldInst m (add offset (ZToReg (4 * i))) = inst.
+
+  Definition containsProgram'(m: Mem mword)(program: list Instruction)(offset: mword) :=
+    regToZ_unsigned offset + 4 * Zlength program <= Memory.memSize m /\
+    decode_prog (Memory.load_word_list m offset (Zlength program)) = program.
+
+  Lemma containsProgram_alt: forall m program offset,
+      containsProgram m program offset <-> containsProgram' m program offset.
+  Proof.
+    intros. unfold containsProgram, containsProgram', decode_prog.
+    intuition idtac.
+    - apply list_elementwise_same_Z. intros i B. specialize (H1 i).
+      assert (0 <= i < Zlength program \/ Zlength program <= i) as C by omega.
+      destruct C as [C | C].
+      + destruct (Znth_error_Some _ program i) as [_ P].
+        specialize (P C).
+        destruct (Znth_error program i) as [inst|] eqn: E; try contradiction.
+        specialize (H1 _ eq_refl). unfold ldInst in H1.
+        erewrite map_Znth_error.
+        * f_equal. eassumption.
+        * apply Znth_error_load_word_list; try assumption.
+      + pose proof (Znth_error_ge_None _ _ C) as P.
+        rewrite P.
+        apply Znth_error_ge_None.
+        rewrite map_Zlength.
+        rewrite Zlength_load_word_list by (apply Zlength_nonneg).
+        assumption.
+    - unfold ldInst. rewrite <- H1 in H.
+      pose proof (map_Znth_error') as P.
+      specialize P with (1 := H).
+      destruct P as [inst' [P Q] ].
+      subst inst.
+      do 2 f_equal.
+      rewrite Znth_error_load_word_list in P.
+      + congruence.
+      + edestruct (Znth_error_Some _ (Memory.load_word_list m offset (Zlength program)))
+          as [Q _].
+        rewrite Zlength_load_word_list in Q by (apply Zlength_nonneg).
+        apply Q. congruence.
+  Qed.
+
+  (* Note: containsProgram for one single [[inst]] could be simplified, but for automation,
+     it's better not to simplify.
+  Lemma containsProgram_cons_inv_old: forall m inst insts offset,
+    containsProgram m (inst :: insts) offset ->
+    containsProgram m [[inst]] offset /\
+    containsProgram m insts (add offset ZToReg 4).
+  Proof.
+    intros *. intro Cp. unfold containsProgram in *. cbn [length] in *.
+    intuition (try omega).
+    + specialize (H0 0). specialize H0 with (1 := eq_refl).
+      intros. destruct i; inverts H1.
+      - assumption.
+      - exfalso. eauto using nth_error_nil_Some.
+    + nat_rel_with_words.
+    + rename H0 into Cp. specialize (Cp (S i)). simpl in Cp.
+      specialize (Cp _ H1).
+      rewrite <- Cp. f_equal.
+      solve_word_eq.
+  Qed.
+  *)
+
+  Definition containsProgram_app_will_work(insts1 insts2: list Instruction)(offset: mword) :=
+    (regToZ_unsigned (mul (add offset (ZToReg 4)) (ZToReg (Zlength insts1))) = 0 ->
+     insts1 = nil \/ insts2 = nil).
+
+  Lemma containsProgram_app_inv0: forall s insts1 insts2 offset,
+    containsProgram s (insts1 ++ insts2) offset ->
+    containsProgram s insts1 offset /\
+    containsProgram s insts2 (add offset (ZToReg (4 * Zlength insts1))) /\
+    containsProgram_app_will_work insts1 insts2 offset.
+  Proof.
+  (*
+    intros *. intro Cp. unfold containsProgram, containsProgram_app_will_work in *.
+    rewrite app_length in Cp.
+    intuition (try nat_rel_with_words).
+    + apply H0. rewrite nth_error_app1; [assumption|].
+      apply nth_error_Some. intro E. rewrite E in H1. discriminate.
+    + rewrite <- (H0 (length insts1 + i)).
+      - f_equal. solve_word_eq.
+      - rewrite nth_error_app2 by omega.
+        replace (length insts1 + i - length insts1) with i by omega.
+        assumption.
+    + destruct insts2; [solve [auto]|].
+      destruct insts1; [solve [auto]|].
+      exfalso.
+      simpl (length _) in *.
+      rewrite Nat.mul_add_distr_l in H.
+      rewrite Nat.add_assoc in H.
+      rewrite wordToNat_wplus in H1.
+      rewrite? wordToNat_wmult in *.
+      rewrite? wordToNat_natToWord_eqn in *.
+      pose proof pow2_wXLEN_4.
+      rewrite Nat.add_mod in H1 by omega.
+      rewrite <- Nat.mul_mod in * by omega.
+      rewrite Nat.add_mod_idemp_r in H1 by omega.
+      rewrite <- Nat.add_mod in H1 by omega.
+      pose proof (Memory.memSize_bound s).
+      rewrite Nat.mod_small in H1 by omega.
+      clear -H1. omega.
+  Qed.
+   *)
+  Admitted.
+
+  Lemma containsProgram_app_inv: forall s insts1 insts2 offset,
+    containsProgram s (insts1 ++ insts2) offset ->
+    containsProgram s insts1 offset /\
+    containsProgram s insts2 (add offset (mul (ZToReg 4) (ZToReg (Zlength insts1)))) /\
+    containsProgram_app_will_work insts1 insts2 offset.
+  Proof.
+    intros.
+    destruct (containsProgram_app_inv0 _ _ H) as [H1 H2].
+    rewrite ZToReg_morphism.(morph_mul) in H2.
+    rewrite <- regToZ_unsigned_four in H2.
+    rewrite ZToReg_regToZ_unsigned in H2.
+    auto.
+  Qed.
+
+  Lemma containsProgram_cons_inv: forall m inst insts offset,
+    containsProgram m (inst :: insts) offset ->
+    containsProgram m [[inst]] offset /\
+    containsProgram m insts (add offset (ZToReg 4)) /\
+    containsProgram_app_will_work [[inst]] insts offset.
+  Proof.
+    intros.
+    pose proof containsProgram_app_inv as P.
+    specialize P with (insts1 := [[inst]]) (insts2 := insts).
+    (* TODO how to automate this nicely? "match" and equate? *)
+    replace (add offset (ZToReg 4)) with (add offset (mul (ZToReg 4) (ZToReg (Zlength [[inst]])))); auto.
+    rewrite Zlength_cons. rewrite Zlength_nil.
+    change (0 + 1) with 1.
+    rewrite <- regToZ_unsigned_one.
+    simpl in *.
+    rewrite ZToReg_regToZ_unsigned.
+    ring.
+  Qed.
+
+  Lemma containsProgram_app: forall m insts1 insts2 offset,
+      containsProgram_app_will_work insts1 insts2 offset ->
+      containsProgram m insts1 offset ->
+      containsProgram m insts2 (add offset (mul (ZToReg 4) (ZToReg (Zlength insts1)))) ->
+      containsProgram m (insts1 ++ insts2) offset.
+  Proof.
+    (*
+    unfold containsProgram, containsProgram_app_will_work.
+    intros *. intro A. intros. rewrite app_length.
+    intuition idtac.
+    - clear H2 H3.
+      repeat match goal with
+             | IsMem: Memory.Memory ?M _, m: ?M |- _ =>
+               unique pose proof (@Memory.memSize_bound M _ IsMem m)
+             end.
+      pose proof pow2_wXLEN_4.
+      assert (let x := regToZ_unsigned  (offset ^+ $ (4) ^* $ (length insts1)) in x = 0 \/ x > 0) as C
+        by (cbv zeta; omega).
+      destruct C as [C | C].
+      + specialize (A C). destruct A as [A | A].
+        * subst insts1.
+          change (length [[]]) with 0 in *.
+          rewrite Nat.add_0_l.
+          replace (offset ^+ $ (4) ^* $ (0)) with offset in C by solve_word_eq.
+          apply wordToNat_zero in C. subst offset.
+          rewrite roundTrip_0 in *.
+          match goal with
+          | H: regToZ_unsigned ?b + 4 * length insts2 <= _ |- _ =>
+            replace 0 with (regToZ_unsigned b) at 1; [assumption|]
+          end.
+          rewrite <- roundTrip_0 at 4.
+          f_equal.
+          solve_word_eq.
+        * subst insts2.
+          change (length [[]]) with 0.
+          rewrite Nat.add_0_r.
+          assumption.
+      + repeat match goal with
+             | IsMem: Memory.Memory ?M _, m: ?M |- _ =>
+               unique pose proof (@Memory.memSize_bound M _ IsMem m)
+             end.
+        pose proof pow2_wXLEN_4.
+        rewrite? wordToNat_wplus in *.
+        rewrite? wordToNat_natToWord_eqn in *.
+        rewrite? wordToNat_wmult in *.
+        rewrite? wordToNat_natToWord_eqn in *.
+        rewrite <- Nat.mul_mod in * by omega.
+        rewrite Nat.add_mod_idemp_r in * by omega.
+        nat_div_mod_to_quot_rem.
+        assert (q = 0 \/ q > 0) as D by omega.
+        destruct D as [D | D]; nia.
+    - assert (i < length insts1 \/ length insts1 <= i) as E by omega.
+      destruct E as [E | E].
+      + rewrite nth_error_app1 in H0 by assumption. eauto.
+      + rewrite nth_error_app2 in H0 by assumption.
+        erewrite <- H3; [|exact H0].
+        f_equal.
+        replace i with (i - length insts1 + length insts1) at 1 by omega.
+        forget (i - length insts1) as i'.
+        solve_word_eq.
+  Qed.*)
+  Admitted.
+
+  Lemma containsProgram_cons: forall m inst insts offset,
+    containsProgram_app_will_work [[inst]] insts offset ->
+    containsProgram m [[inst]] offset ->
+    containsProgram m insts (add offset (ZToReg 4)) ->
+    containsProgram m (inst :: insts) offset.
+  Proof.
+    intros. change (inst :: insts) with ([[inst]] ++ insts).
+    apply containsProgram_app; [assumption..|].
+    rewrite Zlength_cons, Zlength_nil.
+    repeat match goal with
+           | H: containsProgram _ _ ?x |- _ => progress (ring_simplify x in H)
+           | |-  containsProgram _ _ ?x     => progress (ring_simplify x)
+           end.
+    assumption.
+  Qed.
+
+End ContainsProgram.
